src/phase0/litter.lean
@@ -139,6 +139,20 @@ def to_prod (N : near_litter) : litter × set atom := (N.1, N.2)
 lemma to_prod_injective : injective to_prod :=
 by { rintro ⟨i, s⟩ ⟨j, t⟩ h, rw prod.ext_iff at h, exact ext h.1 h.2 }
 
+@[simp] lemma is_near_litter (N : near_litter) (i : litter) : is_near_litter i N ↔ N.fst = i :=
+begin
+  split,
+  { intro h,
+    exact is_near_litter.unique N.snd.prop h, },
+  { intro h,
+    have := h,
+    rw ← h,
+    rw ← is_near_litter_litter_set_iff at h,
+    refine is_near.trans h _,
+    rw ← this,
+    exact N.snd.prop, },
+end
+
 end near_litter
 
 namespace litter
